Ed: Prove PointDecompress

code/experimental/ed25519/Hacl.Impl.Ed25519.PointDecompress.fst
@@ -6,10 +6,14 @@ open FStar.Mul
 
 open Lib.IntTypes
 open Lib.Buffer
+open Lib.ByteSequence
 
 open Hacl.Bignum25519
 
 module F51 = Hacl.Impl.Ed25519.Field51
+
+module SC = Spec.Curve25519
+module SE = Spec.Ed25519
 
 #set-options "--z3rlimit 15 --max_fuel 0 --max_ifuel 0"
 
@@ -18,10 +22,28 @@ val most_significant_bit:
   s:lbuffer uint8 32ul ->
   Stack uint64
     (requires fun h -> live h s)
-    (ensures fun h0 z h1 -> h1 == h0)
+    (ensures fun h0 z h1 -> h0 == h1 /\
+      (v z = 0 \/ v z = 1) /\
+      v z == (nat_from_bytes_le (as_seq h0 s) / pow2 255) % 2
+    )
+
+open FStar.Calc
+
 let most_significant_bit s =
   let s31 = s.(31ul) in
   let z   = s31 >>. 7ul in
+  (**) let h0 = get() in
+  (**) FStar.Math.Lemmas.lemma_div_lt_nat (v s31) 8 7;
+  (**) uints_from_bytes_le_nat_lemma #U8 #SEC #32 (as_seq h0 s);
+  (**) nat_from_intseq_le_slice_lemma (as_seq h0 s) 31;
+  (**) nat_from_intseq_le_lemma0 (Seq.slice (as_seq h0 s) 31 32);
+  (**) assert_norm (31 * 8 == 248);
+  (**) FStar.Math.Lemmas.lemma_div_mod_plus (nat_from_intseq_le (Seq.slice (as_seq h0 s) 0 31))
+    (v s31) (pow2 248);
+  (**) FStar.Math.Lemmas.small_div (nat_from_intseq_le (Seq.slice (as_seq h0 s) 0 31)) (pow2 248);
+  (**) FStar.Math.Lemmas.division_multiplication_lemma (nat_from_bytes_le (as_seq h0 s)) (pow2 248) (pow2 7);
+  (**) assert_norm (pow2 248 * pow2 7 = pow2 255);
+  (**) FStar.Math.Lemmas.small_mod (v s31 / pow2 7) 2;
   to_u64 z
 
 inline_for_extraction noextract
@@ -32,14 +54,22 @@ val point_decompress_:
   Stack bool
     (requires fun h ->
       live h out /\ live h s /\ live h tmp /\
-      disjoint s tmp /\ disjoint out tmp)
-    (ensures  fun h0 b h1 -> modifies (loc out |+| loc tmp) h0 h1)
+      disjoint s tmp /\ disjoint out tmp /\
+      F51.mul_inv_t h (gsub tmp 5ul 5ul)
+    )
+    (ensures  fun h0 b h1 -> modifies (loc out |+| loc tmp) h0 h1 /\
+      (b <==> Some? (SE.point_decompress (as_seq h0 s))) /\
+      (b ==> (F51.point_eval h1 out == Some?.v (SE.point_decompress (as_seq h0 s))))
+    )
+
 let point_decompress_ out s tmp =
   let y    = sub tmp 0ul 5ul in
   let x    = sub tmp 5ul 5ul in
+  let h0 = get() in
   let sign = most_significant_bit s in
-  admit();
+  let h1 = get() in
   load_51 y s;
+  let h2 = get() in
   let z = Hacl.Impl.Ed25519.RecoverX.recover_x x y sign in
 
   let res =
@@ -71,5 +101,4 @@ let point_decompress out s =
   let tmp  = create 10ul (u64 0) in
   let res = point_decompress_ out s tmp in
   pop_frame();
-  admit();
   res
